Move wal proof into a directory

src/program_proof/wal/specs.v
@@ -1,32 +1,10 @@
 From RecordUpdate Require Import RecordSet.
 Import RecordSetNotations.
 
-From Perennial.Helpers Require Import Transitions.
-From Perennial.program_proof Require Import proof_prelude.
 From Goose.github_com.mit_pdos.goose_nfsd Require Import wal.
 
-(* defining the abstraction of the log, including internal abstractions *)
-
-Module update.
-  Record t :=
-    { addr: u64;
-      b: Block; }.
-End update.
-
-Definition disk := gmap Z Block.
-
-Module log_state.
-  Record t :=
-    mk { (* tracks the disk corresponding to each LogPosition (the identifiers
-    handed out by MemAppend) *)
-        txn_disk: gmap u64 disk;
-        (* installed_to promises what will be read after a cache miss *)
-        installed_to: u64;
-        (* durable_to promises what will be on-disk after a crash *)
-        durable_to: u64;
-      }.
-  Global Instance _eta: Settable _ := settable! mk <txn_disk; installed_to; durable_to>.
-End log_state.
+From Perennial.Helpers Require Import Transitions.
+From Perennial.program_proof Require Import proof_prelude wal.abstraction.
 
 Instance gen_gmap_entry {Σ K} `{Countable K} {V} (m: gmap K V) :
   GenPred (K*V) Σ (fun _ '(k, v) => m !! k = Some v).
