src/program_proof/wal/abstraction.v
@@ -1,0 +1,25 @@
+From RecordUpdate Require Import RecordSet.
+Import RecordSetNotations.
+
+From Perennial.program_proof Require Import proof_prelude.
+
+Module update.
+  Record t :=
+    { addr: u64;
+      b: Block; }.
+End update.
+
+Definition disk := gmap Z Block.
+
+Module log_state.
+  Record t :=
+    mk { (* tracks the disk corresponding to each LogPosition (the identifiers
+    handed out by MemAppend) *)
+        txn_disk: gmap u64 disk;
+        (* installed_to promises what will be read after a cache miss *)
+        installed_to: u64;
+        (* durable_to promises what will be on-disk after a crash *)
+        durable_to: u64;
+      }.
+  Global Instance _eta: Settable _ := settable! mk <txn_disk; installed_to; durable_to>.
+End log_state.
